xdsl_smt/dialects/synth_dialect.py
@@ -1,9 +1,12 @@
-from xdsl.ir import Attribute, Dialect, SSAValue
+from xdsl.ir import Attribute, Dialect, SSAValue, Sequence
+from xdsl.dialects.builtin import StringAttr
 from xdsl.irdl import (
     irdl_op_definition,
     IRDLOperation,
+    prop_def,
     result_def,
     operand_def,
+    var_operand_def,
     traits_def,
 )
 from xdsl.traits import Pure
@@ -47,5 +50,18 @@ class ConversionOp(IRDLOperation):
 
     assembly_format = "attr-dict $input `:` type($input) `->` type($output)"
 
+@irdl_op_definition
+class OperationOp(IRDLOperation):
+    name = "synth.op"
 
-SynthDialect = Dialect("synth", [ConstantOp, FromValueOp, ConversionOp])
+    op_name = prop_def()
+
+    res = result_def()
+    ops = var_operand_def()
+
+    def __init__(self, operands: Sequence[SSAValue], res_type: Attribute, op_name: StringAttr):
+        super().__init__(operands=[operands], result_types=[res_type], properties={"op_name": op_name})
+
+    assembly_format = "$op_name $ops attr-dict `:` type($ops) `->` type($res)"
+
+SynthDialect = Dialect("synth", [ConstantOp, FromValueOp, ConversionOp, OperationOp])
