xdsl_smt/semantics/riscv_semantics.py
@@ -38,26 +38,33 @@ class ImmSemantics(AttributeSemantics):
         return op.res
 
 
-@dataclass
-class TrivialRdRsRsIntSemantics(OperationSemantics):
-    riscv_op_type: type[Operation]
-    smt_op_type: type[Operation]
+def regToWord(val: SSAValue, rewriter: PatternRewriter) -> SSAValue:
+    extractOp = smt_bv.ExtractOp(val, WORD_SIZE//2-1, 0)
+    rewriter.insert_op_before_matched_op(extractOp)
+    return extractOp.res
 
-    def get_semantics(
-        self,
-        operands: Sequence[SSAValue],
-        results: Sequence[Attribute],
-        attributes: Mapping[str, Attribute | SSAValue],
-				effect_state: SSAValue | None,
-        rewriter: PatternRewriter,
-    ) -> tuple[Sequence[SSAValue], SSAValue | None]:
-        assert isinstance(results[0], IntRegisterType)
-        new_op = self.smt_op_type.create(
-            operands=operands,
-            result_types=[smt_bv.BitVectorType(WORD_SIZE)],
-        )
-        rewriter.insert_op_before_matched_op([new_op])
-        return ([new_op.results[0]], effect_state)
+def extendTo(val: SSAValue, width : int, rewriter: PatternRewriter, sign : bool = True) -> SSAValue:
+    if sign:
+        extendOp = smt_bv.SignExtendOp(val, smt_bv.BitVectorType(width))
+    else:
+        extendOp = smt_bv.ZeroExtendOp(val, smt_bv.BitVectorType(width))
+    rewriter.insert_op_before_matched_op(extendOp)
+    return extendOp.res
+
+def wordToReg(val: SSAValue, rewriter: PatternRewriter) -> SSAValue:
+    return extendTo(val, WORD_SIZE, rewriter) 
+
+def regToShamt(val: SSAValue, rewriter: PatternRewriter, shamt: int = 6) -> SSAValue:
+    extractOp = smt_bv.ExtractOp(val, shamt-1, 0)
+    rewriter.insert_op_before_matched_op(extractOp)
+    return extractOp.res
+
+def ofBool(val : SSAValue, rewriter : PatternRewriter) -> SSAValue:
+    zero = smt_bv.ConstantOp(0, WORD_SIZE)
+    one = smt_bv.ConstantOp(1, WORD_SIZE)
+    iteOp = smt.IteOp(val, one.res, zero.res) 
+    rewriter.insert_op_before_matched_op([zero, one, iteOp])
+    return iteOp.res
 
 @dataclass
 class RdRsRsIntSemantics(OperationSemantics):
@@ -75,22 +82,28 @@ class RdRsRsIntSemantics(OperationSemantics):
         new_results = self.semantics(operands[0], operands[1], rewriter)
         return (new_results, effect_state)
 
-def ofBool(val : SSAValue, rewriter : PatternRewriter) -> SSAValue:
-    zero = smt_bv.ConstantOp(0, 64)
-    one = smt_bv.ConstantOp(1, 64)
-    iteOp = smt.IteOp(val, one.res, zero.res) 
-    rewriter.insert_op_before_matched_op([zero, one, iteOp])
-    return iteOp.res
-
-def slt_semantics(rs1 : SSAValue, rs2 : SSAValue, rewriter : PatternRewriter) -> Sequence[SSAValue]: 
-    sltOp = smt_bv.SltOp(rs1, rs2)
-    rewriter.insert_op_before_matched_op([sltOp])
-    return [ofBool(sltOp.res, rewriter)]
-
 @dataclass
-class TrivialRdRsImmIntSemantics(OperationSemantics):
-    riscv_op_type: type[Operation]
-    smt_op_type: type[Operation]
+class RdRsRsIntWordSemantics(OperationSemantics):
+    semantics: Callable[[SSAValue, SSAValue, PatternRewriter], Sequence[SSAValue]]
+
+    def get_semantics(
+        self,
+        operands: Sequence[SSAValue],
+        results: Sequence[Attribute],
+        attributes: Mapping[str, Attribute | SSAValue],
+				effect_state: SSAValue | None,
+        rewriter: PatternRewriter,
+    ) -> tuple[Sequence[SSAValue], SSAValue | None]:
+        assert isinstance(results[0], IntRegisterType)
+        rs1 = regToWord(operands[0], rewriter)
+        rs2 = regToWord(operands[1], rewriter)
+        temp_results = self.semantics(rs1, rs2, rewriter)
+        new_results = [wordToReg(temp_results[0], rewriter)]
+        return (new_results, effect_state)
+
+@dataclass 
+class RdRsImmIntSemantics(OperationSemantics):
+    semantics: Callable[[SSAValue, SSAValue, PatternRewriter], Sequence[SSAValue]]
 
     def get_semantics(
         self,
@@ -105,25 +118,181 @@ class TrivialRdRsImmIntSemantics(OperationSemantics):
         if isinstance(imm, Attribute):
             assert isinstance(imm, Attribute)
             imm = ImmSemantics().get_semantics(imm, rewriter)
-        imm_extend = smt_bv.SignExtendOp(imm, smt_bv.BitVectorType(WORD_SIZE))
-        op = self.smt_op_type.create(
-            operands=[operands[0], imm_extend.results[0]],
-            result_types=[smt_bv.BitVectorType(WORD_SIZE)]
-        )
-        rewriter.insert_op_before_matched_op([imm_extend, op])
-        return ([op.results[0]], effect_state)
+        imm = extendTo(imm, WORD_SIZE, rewriter)
+        new_results = self.semantics(operands[0], imm, rewriter)
+        return (new_results, effect_state)
+        
+@dataclass
+class RdRsImmIntWordSemantics(OperationSemantics):
+    semantics: Callable[[SSAValue, SSAValue, PatternRewriter], Sequence[SSAValue]]
+
+    def get_semantics(
+        self,
+        operands: Sequence[SSAValue],
+        results: Sequence[Attribute],
+        attributes: Mapping[str, Attribute | SSAValue],
+				effect_state: SSAValue | None,
+        rewriter: PatternRewriter,
+    ) -> tuple[Sequence[SSAValue], SSAValue | None]:
+        assert isinstance(results[0], IntRegisterType)
+        imm = attributes["immediate"]
+        if isinstance(imm, Attribute):
+            assert isinstance(imm, Attribute)
+            imm = ImmSemantics().get_semantics(imm, rewriter)
+        imm = extendTo(imm, WORD_SIZE, rewriter)
+        temp_results = self.semantics(operands[0], imm, rewriter)
+        trunc_res = regToWord(temp_results[0], rewriter)
+        new_results = [wordToReg(trunc_res, rewriter)]
+        return (new_results, effect_state)
+
+
+@dataclass
+class RdRsRsShamtSemantics(OperationSemantics):
+    semantics: Callable[[SSAValue, SSAValue, PatternRewriter], Sequence[SSAValue]]
+
+    def get_semantics(
+        self,
+        operands: Sequence[SSAValue],
+        results: Sequence[Attribute],
+        attributes: Mapping[str, Attribute | SSAValue],
+		effect_state: SSAValue | None,
+        rewriter: PatternRewriter,
+    ) -> tuple[Sequence[SSAValue], SSAValue | None]:
+        assert isinstance(results[0], IntRegisterType)
+        shamt = regToShamt(operands[1], rewriter)
+        shamt = extendTo(shamt, WORD_SIZE, rewriter, False)
+        new_results = self.semantics(operands[0], shamt, rewriter)
+        return (new_results, effect_state)
+
+@dataclass
+class RdRsRsShamtWordSemantics(OperationSemantics):
+    semantics: Callable[[SSAValue, SSAValue, PatternRewriter], Sequence[SSAValue]]
+
+    def get_semantics(
+        self,
+        operands: Sequence[SSAValue],
+        results: Sequence[Attribute],
+        attributes: Mapping[str, Attribute | SSAValue],
+		effect_state: SSAValue | None,
+        rewriter: PatternRewriter,
+    ) -> tuple[Sequence[SSAValue], SSAValue | None]:
+        assert isinstance(results[0], IntRegisterType)
+        rs1 = regToWord(operands[0], rewriter)
+        shamt = regToShamt(operands[1], rewriter, 5)
+        shamt = extendTo(shamt, WORD_SIZE//2, rewriter, False)
+        temp_results = self.semantics(rs1, shamt, rewriter)
+        new_results = [wordToReg(temp_results[0], rewriter)]
+        return (new_results, effect_state)
+
+
+@dataclass 
+class RdRsShamtSemantics(OperationSemantics):
+    semantics: Callable[[SSAValue, SSAValue, PatternRewriter], Sequence[SSAValue]]
+
+    def get_semantics(
+        self,
+        operands: Sequence[SSAValue],
+        results: Sequence[Attribute],
+        attributes: Mapping[str, Attribute | SSAValue],
+		effect_state: SSAValue | None,
+        rewriter: PatternRewriter,
+    ) -> tuple[Sequence[SSAValue], SSAValue | None]:
+        assert isinstance(results[0], IntRegisterType)
+        shamt = attributes["immediate"]
+        if isinstance(shamt, Attribute):
+            assert isinstance(shamt, Attribute)
+            shamt = ImmSemantics().get_semantics(shamt, rewriter)
+        shamt = extendTo(shamt, WORD_SIZE, rewriter, False)
+        new_results = self.semantics(operands[0], shamt, rewriter)
+        return (new_results, effect_state)
+
+@dataclass 
+class RdRsShamtWordSemantics(OperationSemantics):
+    semantics: Callable[[SSAValue, SSAValue, PatternRewriter], Sequence[SSAValue]]
+
+    def get_semantics(
+        self,
+        operands: Sequence[SSAValue],
+        results: Sequence[Attribute],
+        attributes: Mapping[str, Attribute | SSAValue],
+		effect_state: SSAValue | None,
+        rewriter: PatternRewriter,
+    ) -> tuple[Sequence[SSAValue], SSAValue | None]:
+        assert isinstance(results[0], IntRegisterType)
+        shamt = attributes["immediate"]
+        if isinstance(shamt, Attribute):
+            assert isinstance(shamt, Attribute)
+            shamt = ImmSemantics().get_semantics(shamt, rewriter)
+        rs1 = regToWord(operands[0], rewriter)
+        shamt = extendTo(shamt, WORD_SIZE//2, rewriter, False)
+        temp_results = self.semantics(rs1, shamt, rewriter)
+        new_results = [wordToReg(temp_results[0], rewriter)]
+        return (new_results, effect_state)
+
+def trivial_binary_semantics(op_type : type[smt_bv.BinaryBVOp]
+    ) -> Callable[[SSAValue, SSAValue, PatternRewriter], Sequence[SSAValue]]:
+    def semantics(operand1 : SSAValue, operand2: SSAValue, rewriter: PatternRewriter) -> Sequence[SSAValue]:
+        op = op_type(operand1, operand2)
+        rewriter.insert_op_before_matched_op(op)
+        return [op.res]
+    return semantics
+
+def cmp_semantics(op_type: type[smt_bv.BinaryPredBVOp]):
+    def semantics(rs1 : SSAValue, rs2 : SSAValue, rewriter : PatternRewriter) -> Sequence[SSAValue]: 
+        cmpOp = op_type(rs1, rs2)
+        rewriter.insert_op_before_matched_op([cmpOp])
+        return [ofBool(cmpOp.res, rewriter)]
+    return semantics
+
+
+add_semantics = trivial_binary_semantics(smt_bv.AddOp)
+
+sll_semantics = trivial_binary_semantics(smt_bv.ShlOp)
+srl_semantics = trivial_binary_semantics(smt_bv.LShrOp)
+sra_semantics = trivial_binary_semantics(smt_bv.AShrOp)
+
+def slliuw_semantics(rs : SSAValue, shamt : SSAValue, rewriter : PatternRewriter) -> Sequence[SSAValue]:
+    trunc = regToWord(rs, rewriter)
+    zero_ext = smt_bv.ZeroExtendOp(trunc, smt_bv.BitVectorType(64)) 
+    shift = smt_bv.ShlOp(zero_ext.res, shamt)
+    rewriter.insert_op_before_matched_op([zero_ext, shift])
+    return [shift.res]
 
 riscv_semantics: dict[type[Operation], OperationSemantics] = {
-    riscv.AddOp : TrivialRdRsRsIntSemantics(riscv.AddOp, smt_bv.AddOp),
-    riscv.SubOp : TrivialRdRsRsIntSemantics(riscv.SubOp, smt_bv.SubOp),
-    riscv.XorOp : TrivialRdRsRsIntSemantics(riscv.XorOp, smt_bv.XorOp),
-    riscv.AndOp : TrivialRdRsRsIntSemantics(riscv.AndOp, smt_bv.AndOp),
-    riscv.OrOp : TrivialRdRsRsIntSemantics(riscv.OrOp, smt_bv.OrOp),
+    riscv.AddOp : RdRsRsIntSemantics(add_semantics),
+    riscv.AddiOp : RdRsImmIntSemantics(add_semantics),
+    riscv.AddwOp : RdRsRsIntWordSemantics(add_semantics),
+    riscv.AddiwOp : RdRsImmIntWordSemantics(add_semantics),
 
-    riscv.AddiOp : TrivialRdRsImmIntSemantics(riscv.AddiOp, smt_bv.AddOp),
-    riscv.XoriOp : TrivialRdRsImmIntSemantics(riscv.XoriOp, smt_bv.XorOp),
-    riscv.AndiOp : TrivialRdRsImmIntSemantics(riscv.AndiOp, smt_bv.AndOp),
-    riscv.OriOp : TrivialRdRsImmIntSemantics(riscv.OriOp, smt_bv.OrOp),
+    riscv.SubOp : RdRsRsIntSemantics(trivial_binary_semantics(smt_bv.SubOp)),
+    riscv.SubwOp : RdRsRsIntWordSemantics(trivial_binary_semantics(smt_bv.SubOp)),
 
-    riscv.SltOp: RdRsRsIntSemantics(slt_semantics),
+    riscv.XorOp : RdRsRsIntSemantics(trivial_binary_semantics(smt_bv.XorOp)),
+    riscv.AndOp : RdRsRsIntSemantics(trivial_binary_semantics(smt_bv.AndOp)),
+    riscv.OrOp : RdRsRsIntSemantics(trivial_binary_semantics(smt_bv.OrOp)),
+
+    riscv.XoriOp : RdRsImmIntSemantics(trivial_binary_semantics(smt_bv.XorOp)),
+    riscv.AndiOp : RdRsImmIntSemantics(trivial_binary_semantics(smt_bv.AndOp)),
+    riscv.OriOp : RdRsImmIntSemantics(trivial_binary_semantics(smt_bv.OrOp)),
+
+    riscv.SltOp: RdRsRsIntSemantics(cmp_semantics(smt_bv.SltOp)),
+    riscv.SltiOp: RdRsImmIntSemantics(cmp_semantics(smt_bv.SltOp)),
+    riscv.SltuOp: RdRsRsIntSemantics(cmp_semantics(smt_bv.UltOp)),
+    riscv.SltiuOp: RdRsImmIntSemantics(cmp_semantics(smt_bv.UltOp)),
+
+    riscv.SllOp: RdRsRsShamtSemantics(sll_semantics),
+    riscv.SlliOp: RdRsShamtSemantics(sll_semantics),
+    riscv.SllwOp: RdRsRsShamtWordSemantics(sll_semantics),
+    riscv.SlliwOp: RdRsShamtWordSemantics(sll_semantics),
+    riscv.SlliUwOp: RdRsShamtSemantics(slliuw_semantics),
+    
+    riscv.SrlOp: RdRsRsShamtSemantics(srl_semantics),
+    riscv.SrliOp: RdRsShamtSemantics(srl_semantics),
+    riscv.SrlwOp: RdRsRsShamtWordSemantics(srl_semantics),
+    riscv.SrliwOp: RdRsShamtWordSemantics(srl_semantics),
+
+    riscv.SraOp: RdRsRsShamtSemantics(sra_semantics),
+    riscv.SraiOp: RdRsShamtSemantics(sra_semantics),
+    riscv.SrawOp: RdRsRsShamtWordSemantics(sra_semantics),
+    riscv.SraiwOp: RdRsShamtWordSemantics(sra_semantics),
 }
