xdsl_smt/utils/proofs/lean_printer.py
@@ -2,6 +2,7 @@ from abc import abstractmethod, ABC
 from dataclasses import dataclass
 
 from xdsl.ir import Operation, SSAValue, Block, TypeAttribute
+from xdsl.dialects.builtin import IntAttr
 
 from xdsl_smt.dialects import smt_bitvector_dialect as smt_bv
 from xdsl.dialects.smt import BitVectorType, BoolType
@@ -9,7 +10,7 @@ from xdsl_smt.semantics.riscv_semantics import *
 
 class IdDict:
     id = 0
-    ids : Mapping[SSAValue, int] = {}
+    ids : dict[SSAValue, int] = {}
     def get_id(self, value: SSAValue) -> int:
         if value not in self.ids:
             self.ids[value] = self.id
@@ -27,12 +28,13 @@ def get_type(type : TypeAttribute) -> str:
 class LeanPrintable(ABC):
       
     @abstractmethod
-    def print(self, op : Operation, ids : IdDict, indent=0) : pass
+    def print(self, op : Operation, ids : IdDict, indent : int = 0) : pass
 
 class ConstantOp(LeanPrintable):
 
-    def print(self, op : Operation, ids : IdDict, indent=0) :
+    def print(self, op : Operation, ids : IdDict, indent:int = 0) :
         assert isinstance(op, smt_bv.ConstantOp)
+        assert isinstance(op.result_types[0], TypeAttribute)
         print("{}let a{} : {} := {} ;".format(
             "  "*indent,
             ids.get_id(op.res),
@@ -45,11 +47,31 @@ class BinaryOp(LeanPrintable):
     smt_op_type: type[Operation]
     lean_function_name: str
 
-    def print(self, op : Operation, ids : IdDict, indent=0):
+    def print(self, op : Operation, ids : IdDict, indent : int = 0):
         assert type(op) == self.smt_op_type
-        rtype = op.result_types[0]
+        rtype  = op.result_types[0]
+        assert isinstance(rtype, TypeAttribute)
         res, op1, op2 = op.results[0], op.operands[0], op.operands[1]
         print("{}let a{} : {} := ({} a{} a{}) ;".format(
+            "  "*indent,
+            ids.get_id(res),
+            get_type(rtype),
+            self.lean_function_name,
+            ids.get_id(op1),
+            ids.get_id(op2), 
+        ))
+
+@dataclass
+class ShiftOp(LeanPrintable):
+    smt_op_type: type[Operation]
+    lean_function_name: str
+
+    def print(self, op : Operation, ids : IdDict, indent : int = 0):
+        assert type(op) == self.smt_op_type
+        rtype  = op.result_types[0]
+        assert isinstance(rtype, TypeAttribute)
+        res, op1, op2 = op.results[0], op.operands[0], op.operands[1]
+        print("{}let a{} : {} := ({} a{} (BitVec.toNat a{})) ;".format(
             "  "*indent,
             ids.get_id(res),
             get_type(rtype),
@@ -63,9 +85,10 @@ class TernaryOp(LeanPrintable):
     smt_op_type: type[Operation]
     lean_function_name: str
 
-    def print(self, op : Operation, ids : IdDict, indent=0):
+    def print(self, op : Operation, ids : IdDict, indent : int = 0):
         assert type(op) == self.smt_op_type
         rtype = op.result_types[0]
+        assert isinstance(rtype, TypeAttribute)
         res, op1, op2, op3 = op.results[0], op.operands[0], op.operands[1], op.operands[2]
         print("{}let a{} : {} := ({} a{} a{} a{}) ;".format(
             "  "*indent,
@@ -82,7 +105,7 @@ class ExtendOp(LeanPrintable):
 
     mode : str 
 
-    def print(self, op : Operation, ids : IdDict, indent=0):
+    def print(self, op : Operation, ids : IdDict, indent : int = 0):
         assert isinstance(rtype := op.result_types[0], BitVectorType)
         print("{}let a{} : {} := (BitVec.{}Extend {} a{}) ;".format(
             "  "*indent,
@@ -93,14 +116,40 @@ class ExtendOp(LeanPrintable):
             ids.get_id(op.operands[0]),
         ))
 
-op_printers = {
+@dataclass 
+class ExtractOp(LeanPrintable):
+
+    def print(self, op : Operation, ids : IdDict, indent : int = 0):
+        rtype = op.result_types[0]
+        assert isinstance(rtype, TypeAttribute)
+        res, op1 = op.results[0], op.operands[0]
+        end, start = op.attributes["end"], op.attributes["start"]
+        assert isinstance(end, IntAttr)
+        assert isinstance(start, IntAttr)
+        print("{}let a{} : {} := ({} {} {} a{}) ;".format(
+            "  "*indent,
+            ids.get_id(res),
+            get_type(rtype),
+            "BitVec.extractLsb",
+            end.data,
+            start.data, 
+            ids.get_id(op1),
+        ))
+
+op_printers : dict[type[Operation], LeanPrintable] = {
     smt_bv.AddOp : BinaryOp(smt_bv.AddOp, "BitVec.add"),
+    smt_bv.SubOp : BinaryOp(smt_bv.SubOp, "BitVec.sub"),
     smt_bv.OrOp : BinaryOp(smt_bv.OrOp, "BitVec.or"),
     smt_bv.AndOp : BinaryOp(smt_bv.AndOp, "BitVec.and"),
     smt_bv.XorOp : BinaryOp(smt_bv.XorOp, "BitVec.xor"),
     smt_bv.SignExtendOp : ExtendOp("sign"),
     smt_bv.ZeroExtendOp : ExtendOp("zero"),
     smt_bv.SltOp : BinaryOp(smt_bv.SltOp, "BitVec.slt"),
+    smt_bv.UltOp : BinaryOp(smt_bv.UltOp, "BitVec.ult"),
+    smt_bv.ShlOp : ShiftOp(smt_bv.ShlOp, "BitVec.shiftLeft"),
+    smt_bv.LShrOp : ShiftOp(smt_bv.LShrOp, "BitVec.ushiftRight"),
+    smt_bv.AShrOp : ShiftOp(smt_bv.AShrOp, "BitVec.sshiftRight"),
+    smt_bv.ExtractOp : ExtractOp(),
     smt.IteOp : TernaryOp(smt.IteOp, "cond"),
     smt_bv.ConstantOp : ConstantOp()
 }
@@ -112,9 +161,11 @@ def print_lean_theorem(name : str, block: Block, results: Sequence[SSAValue]) ->
     args = ""
 
     for arg in block.args:
+        assert isinstance(arg.type, TypeAttribute)
         args += f"a{ids.get_id(arg)} "
         typed_args += f"(a{ids.get_id(arg)} : {get_type(arg.type)}) "
 
+    assert isinstance(results[0].type, TypeAttribute)
     print(f"def _{name} {typed_args}: {get_type(results[0].type)} :=")
     for op in block.walk():
         if type(op) not in op_printers:
@@ -122,5 +173,5 @@ def print_lean_theorem(name : str, block: Block, results: Sequence[SSAValue]) ->
         op_printers[type(op)].print(op, ids, indent=1) 
     print(f"  a{ids.get_id(results[0])}")
     print(f"theorem {name}_eq {typed_args}: RV64.{name} {args}= _{name} {args}:= by")
-    print(f"  simp [RV64.{name}, _{name}]")
-    print("  try bv_decide")
+    print(f"  unfold RV64.{name} _{name}")
+    print("  bv_decide")
