xdsl_smt/utils/proofs/print_equivalence_theorems.py
@@ -1,0 +1,60 @@
+from xdsl.dialects import riscv
+
+from xdsl_smt.semantics.riscv_semantics import *
+from riscv_instructions_smt import *
+from lean_printer import print_lean_theorem
+
+def print_theorem(name : str, semantics : tuple[Block, Sequence[SSAValue]]):
+    block, res = semantics 
+    print_lean_theorem(name, block, res)
+
+rdrsrs : Sequence[type[Operation]] = [ 
+    riscv.AddOp,
+    riscv.AddwOp,
+    riscv.SubOp,
+    riscv.SubwOp,
+    riscv.OrOp,
+    riscv.XorOp,
+    riscv.AndOp,
+    riscv.SltOp,
+    riscv.SltuOp,
+    riscv.SllOp,
+    riscv.SllwOp,
+    riscv.SrlOp,
+    riscv.SrlwOp,
+    riscv.SraOp,
+    riscv.SrawOp,
+]
+
+rdrsimm : Sequence[type[Operation]] = [
+    riscv.AddiOp,
+    riscv.AddiwOp,
+    riscv.AndiOp,
+    riscv.OriOp,
+    riscv.XoriOp,
+    riscv.SltiOp,
+    riscv.SltiuOp,
+]
+rdrsshamt : Sequence[tuple[type[Operation], int]] = [
+    (riscv.SlliOp, 6),
+    (riscv.SlliwOp, 5),
+    (riscv.SrliOp, 6),
+    (riscv.SrliwOp, 5),
+    (riscv.SraiOp, 6),
+    (riscv.SraiwOp, 5),
+
+]
+
+
+for op_type in rdrsrs : 
+    print_theorem(op_type.name[6:], rdrsrs_int_op_smt(op_type))
+
+for op_type in rdrsimm : 
+    print_theorem(op_type.name[6:], rdrsimm_int_op_smt(op_type, 12))
+
+for op_type, width in rdrsshamt : 
+    print_theorem(op_type.name[6:], rdrsimm_int_op_smt(op_type, width))
+
+print_theorem("slliuw", rdrsimm_int_op_smt(riscv.SlliUwOp, 6))
+
+
