xdsl_smt/utils/proofs/riscv_instructions_smt.py
@@ -1,4 +1,4 @@
-from xdsl.ir import Operation, SSAValue, Block, BlockArgument
+from xdsl.ir import Operation, SSAValue, Block
 from xdsl.pattern_rewriter import PatternRewriter
 
 from xdsl.dialects.riscv import IntRegisterType
@@ -12,43 +12,35 @@ SMTLowerer.type_lowerers = {
     IntRegisterType: IntRegisterTypeSemantics(),
 }
 
-def lower_block_args(block : Block) -> BlockArgument[Attribute] :
+def lower_block_args(block : Block) :
     for index, arg in enumerate(block.args): 
         new_type = SMTLowerer.lower_type(arg.type)
         new_arg = arg.block.insert_arg(new_type, index)
         arg.replace_by(new_arg)
         arg.block.erase_arg(arg)
 
-def trivial_rdrsrs_int_op_smt(
-        riscv_op_type : type[Operation], 
-        smt_op_type: type[Operation],
-    ) -> tuple[Block, Sequence[SSAValue]]:
-        mock_op = riscv_op_type.create(result_types=[IntRegisterType.unallocated()])
-        block = Block(ops=[mock_op], arg_types=(IntRegisterType.unallocated(), IntRegisterType.unallocated()))
-        rewriter = PatternRewriter(mock_op)
-        lower_block_args(block)
-        a0, a1 = block.args
-        new_res, _ = TrivialRdRsRsIntSemantics(riscv_op_type, smt_op_type).get_semantics([a0, a1], [IntRegisterType.unallocated()], {}, None, rewriter)
-        rewriter.replace_matched_op([], new_res)
-        return block, new_res
 
 def rdrsrs_int_op_smt(
         riscv_op_type : type[Operation], 
-        semantics: Callable[[SSAValue, SSAValue, PatternRewriter], Sequence[SSAValue]]
     ) -> tuple[Block, Sequence[SSAValue]]:
         mock_op = riscv_op_type.create(result_types=[IntRegisterType.unallocated()])
         block = Block(ops=[mock_op], arg_types=(IntRegisterType.unallocated(), IntRegisterType.unallocated()))
         rewriter = PatternRewriter(mock_op)
         lower_block_args(block)
         rhs, lhs = block.args
-        new_res, _ = RdRsRsIntSemantics(semantics).get_semantics([lhs, rhs], [IntRegisterType.unallocated()], {}, None, rewriter)
+        new_res, _ = riscv_semantics[riscv_op_type].get_semantics(
+            [lhs, rhs],
+            [IntRegisterType.unallocated()], 
+            {}, 
+            None, 
+            rewriter
+        )
         rewriter.replace_matched_op([], new_res)
         return block, new_res
 
-def trivial_rdrsimm_int_op_smt(
+def rdrsimm_int_op_smt(
         riscv_op_type : type[Operation], 
-        smt_op_type: type[Operation],
-        width
+        width : int
     ) -> tuple[Block, Sequence[SSAValue]]:
         mock_op = riscv_op_type.create(result_types=[IntRegisterType.unallocated()])
         # The lean definitions I'm using have the immediate as the first argument
@@ -57,6 +49,12 @@ def trivial_rdrsimm_int_op_smt(
 
         rewriter = PatternRewriter(mock_op)
         imm, a0 = block.args
-        new_res, _ = TrivialRdRsImmIntSemantics(riscv_op_type, smt_op_type).get_semantics([a0], [IntRegisterType.unallocated()], {"immediate" : imm}, None, rewriter)
+        new_res, _ = riscv_semantics[riscv_op_type].get_semantics(
+            [a0],
+            [IntRegisterType.unallocated()], 
+            {"immediate" : imm}, 
+            None, 
+            rewriter
+        )
         rewriter.replace_matched_op([], new_res)
         return block, new_res
